proof/examples/zk/abstract/Abstract_exp_proof_8.ec
@@ -18,8 +18,6 @@ module M8 = {
   }  
 }.
 
-
-
 lemma exp_real_speac2 :
  equiv[ M8.expm_spec ~ M1.expm_spec   : arg{1}.`1 = arg{2}.`1 /\  valR arg{1}.`2 = bs2int arg{2}.`2 ==> ={res}] .
 proc. skip. progress.
@@ -31,7 +29,6 @@ qed.
 section.
 declare module M <: BasicOps.
 
-
 declare axiom exp_swap :
  equiv[ M.swapr ~ Spec.swapr    : arg{2}.`1 = arg{1}.`1 /\ arg{2}.`2 = arg{1}.`2 /\   arg{1}.`3 = as_w64 arg{2}.`3
     ==> ={res}].
@@ -39,6 +36,10 @@ declare axiom exp_swap :
 declare axiom exp_ithbit :
  equiv[ M.ith_bit ~ Spec.ith_bit    : arg{2}.`1 = arg{1}.`1 /\  arg{2}.`2 = W64.to_uint arg{1}.`2 
     /\ 0 <= ctr{2} < Rsize ==> ={res} /\ (res{2} = W64.one \/ res{2} = W64.zero) ].
+
+
+declare axiom exp_mulm :
+  equiv [ M.mulm ~ Spec.mul: arg{1}.`2 = arg{2}.`1 /\ arg{1}.`3 = arg{2}.`2 /\ ImplR p{1} P /\ valR a{1} < P /\ valR b{1} < P ==> ={res} /\ valR res{1} < P  ].
 
 
 declare axiom stateless_M (x y : glob M) : x = y.
@@ -79,27 +80,28 @@ transitivity M4.expm
 (valR arg{2}.`1 = P 
    /\  arg{1}.`1 = arg{2}.`2
    /\ arg{1}.`2 = arg{2}.`3
+   /\ valR x{1} < P
      ==> ={res} ).
 progress. 
 exists (x{1} , ( n{2})). progress. 
 smt (bitsR_prop).
 smt(Rsize_pos). auto.
 conseq exp_3_4_1.
-
 transitivity M5.expm
   (={arg} ==> ={res})
   (valR arg{2}.`1 = P 
    /\  arg{1}.`1 = arg{2}.`2
    /\ arg{1}.`2 = arg{2}.`3
+   /\ valR x{1} < P
      ==> ={res} ).
 progress. 
 exists (x{1} , ( n{2})). progress.  smt(). auto.
 conseq exp_4_5.  
 transitivity M6(M).expm
- (arg{2}.`2 = arg{1}.`1 /\ arg{2}.`3 = arg{1}.`2 /\  valR m{2} = P ==> ={res})
+ (arg{2}.`2 = arg{1}.`1 /\ arg{2}.`3 = arg{1}.`2 /\  valR m{2} = P /\ valR x{1} < P ==> ={res})
   (={arg} ==> ={res}).
 progress. smt(). smt().
-conseq (exp_5_6 M exp_swap exp_ithbit _).  admit.
+conseq (exp_5_6 M exp_swap exp_ithbit exp_mulm stateless_M).   smt().
 conseq (exp_6_7 M).
 smt (stateless_M).
 qed.
@@ -109,102 +111,3 @@ end section.
 
 
 
-
-(* declare axiom exp_mulm :  *)
-(*   equiv [ M.mulm ~ Spec.mulm: valR arg{1}.`2 = asint arg{2}.`1 /\ valR arg{1}.`3 = asint arg{2}.`2 /\ ImplR p{1} P  ==> valR res{1} = asint res{2} ]. *)
-
-(* lemma exp_mulm2 :  *)
-(*   equiv [ M.mulm ~ Spec.mul: arg{1}.`2 = arg{2}.`1 /\ arg{1}.`3 = arg{2}.`2 /\ ImplR p{1} P /\ valR a{1} < P /\ valR b{1} < P  ==> ={res} ]. *)
-(* transitivity Spec.mulm *)
-(*      (valR arg{1}.`2 = asint arg{2}.`1 /\ valR arg{1}.`3 = asint arg{2}.`2 /\ ImplR p{1} P   ==> valR res{1} = asint res{2}) *)
-(*      (valR arg{2}.`1 = asint arg{1}.`1 /\ valR arg{2}.`2 = asint arg{1}.`2   ==> valR res{2} = asint res{1}). *)
-(* progress.  *)
-(* exists (inzp (valR a{1}), inzp (valR b{1}) ). progress. *)
-(* smt. smt. smt. smt. *)
-(* progress. smt. *)
-(* conseq exp_mulm.  *)
-(* proc. wp. skip. progress. *)
-(* have  ->: valR (a{2} *** b{2}) = valR a{2} * valR b{2} %% P. smt. *)
-(* have ->: asint (a{1} * b{1}) = asint (a{1})  * asint  b{1} %% P. smt.  *)
-(* smt(). *)
-(* qed. *)
-
-
-(* import Zp. *)
-
-(* lemma kk :  forall (n : int), 0 <= n => forall (a : zp) (b : R), valR b < P => *)
-(*   ImplFp b a => *)
-(*   ImplFp (b ^ n) (inzp (asint a ^ n)). *)
-(* apply intind. progress.  *)
-(* rewrite exp_prop1. *)
-(* have -> : (asint a ^ 0) = 1. smt. *)
-(* rewrite /asint. *)
-(* have -> : (Sub.val (inzp 1))%Sub = 1. smt. *)
-(* smt(valR_one). *)
-(* progress. *)
-(* have ->: (b ^ (i + 1)) = b *** (b ^ i). *)
-(* rewrite exp_prop3. auto. auto.  auto. *)
-(* rewrite exp_prop2. *)
-(* rewrite exp_prop7. auto. *)
-(* have ->: inzp (asint a ^ (i + 1)) =  inzp (asint a * (asint a ^ i)). *)
-(* smt. *)
-(* have ->:  inzp (asint a * (asint a ^ i)) = (inzp (asint a)) * (inzp (asint a ^ i)). *)
-(* smt. *)
-(* rewrite - H2. *)
-(* have ->: asint (inzp (valR b) * inzp (valR b ^ i)) *)
-(*   = (asint (inzp (valR b)) * (asint  (inzp (valR b ^ i)))) %% P. *)
-(* smt. *)
-(* have ih :  ImplFp (b ^ i)  (inzp (valR b ^ i)). *)
-(* rewrite H2. apply H0. auto. auto. *)
-(* rewrite - ih. *)
-(* have ->: asint (inzp (valR b)) = valR b. smt. *)
-(* have ->: valR (b *** (b ^ i)) =  (valR b) * (valR (b ^ i)) %%P. *)
-(* rewrite  to_uintP /=. done. *)
-(* auto. *)
-(* qed. *)
-
-
-(* lemma exp_real_speacc : *)
-(*  equiv[ Spec.expm ~ M8.expm_spec  :  *)
-(*     ImplFp arg{2}.`1 arg{1}.`1 /\ valR arg{2}.`2 = arg{1}.`2 /\ valR x{2} < P ==> ImplFp res{2} res{1}]. *)
-(* proc.  *)
-(* wp.  skip.  progress. *)
-(* apply kk. *)
-(* smt. auto. *)
-(* auto. *)
-(* qed. *)
-
-
-
-(* lemma exp_pre_fin : *)
-(*  equiv[ Spec.expm ~ M7(M).expm  :  *)
-(*        valR arg{2}.`1  = P  *)
-(*    /\  ImplFp  arg{2}.`2 arg{1}.`1 *)
-(*    /\  arg{1}.`2 =  valR arg{2}.`3 *)
-(*      ==> ImplFp res{2} res{1} ]. *)
-(* transitivity M8.expm_spec *)
-(*   (ImplFp arg{2}.`1 arg{1}.`1 /\ valR arg{2}.`2 = arg{1}.`2 /\ valR x{2} < P ==> ImplFp res{2} res{1}) *)
-(*   (valR arg{2}.`1 = P  *)
-(*    /\  arg{1}.`1 = arg{2}.`2 *)
-(*    /\  arg{1}.`2 =  arg{2}.`3 *)
-(*    /\ valR x{1} < P *)
-(*      ==> ={res}). *)
-(* progress. exists (x{2},n{2}). progress. smt(). smt.  smt. auto. *)
-(* conseq exp_real_speacc.    *)
-(* transitivity M1.expm_spec   *)
-(*   (arg{1}.`1 = arg{2}.`1 /\ valR arg{1}.`2 = bs2int arg{2}.`2 /\ valR x{2} < P ==> ={res}) *)
-(*   (valR arg{2}.`1 = P  *)
-(*    /\  arg{1}.`1 = arg{2}.`2 *)
-(*    /\ bs2int arg{1}.`2 = valR arg{2}.`3 *)
-(*    /\ size arg{1}.`2 = Rsize *)
-(*    /\ valR x{1} < P *)
-(*      ==> ={res}). *)
-(* progress.  *)
-(* exists (x{1},  Rbits n{2}). *)
-(* progress. *)
-(* smt(). *)
-(* smt(iii). *)
-(* smt(). *)
-(* conseq exp_real_speac2.  *)
-(* progress. conseq exp_real_speac. *)
-(* qed. *)
